RegEx/RegEx/brzozowski_mem1.lean
@@ -1,0 +1,405 @@
+import Mathlib.Tactic.Basic --for Type*
+import Mathlib.Data.List.Basic
+import Mathlib.Data.Set.Basic
+import «RegEx».Language.language
+import «RegEx».Language.derivative
+import «RegEx».denotational
+import «RegEx».brzozowski
+
+variable [deq𝒜: DecidableEq 𝒜]
+
+/--!
+# Boolean nullability
+
+- `δ` is nice however it produces regexes which are complex: ε ⋅ ε, ε ⋃ ε,
+  which is fine denotationally, but they are not structurally equal to ε.
+
+- νB is a boolean version of ν, maps a regex to true if the empty word is in the language of the regex.
+  This allows us to define the membership function w ∈ R, without quotient types on the regexes (equality modulo an equivance relation).
+  Of course this approch is not at all economical, but it is a first step towards the Brzozowski derivative.
+-/
+@[simp]
+def νB: Regex 𝒜 → Bool
+| Φ => false
+| τ _ => false
+| e₁ ⋅ e₂ => νB e₁ && νB e₂
+| e₁ ⋃ e₂ => νB e₁ || νB e₂
+| _★ => true
+
+theorem νB_correct(e: Regex 𝒜): νB e = true ↔ [] ∈ ℒ e := by {
+  induction e with
+  | empty | token t => tauto
+  | concatenation e₁ e₂ ihe₁ ihe₂ =>
+    simp [ℒ, νB]
+    rw [ihe₁, ihe₂]
+  | union e₁ e₂ ihe₁ ihe₂ =>
+    simp [ℒ, νB]
+    rw [ihe₁, ihe₂]
+  | star e _ =>
+    simp [ℒ, νB, eps_mem_kstar]
+}
+
+theorem νB_false(e: Regex 𝒜): νB e = false ↔ [] ∉ ℒ e := by {
+  rw [←νB_correct]
+  --exact not_iff_not_of_iff (νB_correct e)
+  constructor
+  . intro H
+    rw [H]
+    tauto
+  . induction e with
+    | empty | token t => tauto
+    | concatenation e₁ e₂ ihe₁ ihe₂ =>
+      simp [νB]; tauto
+    | union e₁ e₂ ihe₁ ihe₂ => simp [νB]; tauto
+    | star _ _ => simp [νB]
+}
+/--!
+# Membership is nullable derivative
+-/
+def brzozowski_mem' : Word 𝒜 → Regex 𝒜 → Prop
+  | [], R => νB R
+  | h :: t, R => brzozowski_mem' t (𝒟 h R)
+
+instance brzozowski_membership': Membership (Word 𝒜) (Regex 𝒜) := ⟨brzozowski_mem'⟩
+
+lemma brzozowski_mem'_cons(c: 𝒜)(w: Word 𝒜)(R: Regex 𝒜):
+  (c::w) ∈ R ↔ w ∈ (𝒟 c R)
+:= by rfl
+
+lemma brzozowski_mem'_empty(w: Word 𝒜):
+  w ∉ (Φ: Regex 𝒜)
+:= by {
+  induction w with
+  | nil => simp [Membership.mem, brzozowski_mem'] at *
+  | cons _ _ ih =>
+    simp [ brzozowski_mem', νB] at *
+    exact ih
+}
+
+lemma brzozowski_mem'_union_iff(R₁ R₂ : Regex 𝒜) (w : Word 𝒜):
+  w ∈ (R₁ ⋃ R₂) ↔ w ∈ R₁ ∨ w ∈ R₂
+:= by {
+  induction' w with a x ih generalizing R₁ R₂
+  case nil =>
+    simp [Membership.mem, brzozowski_mem', D_union] at *
+  . simp [Membership.mem, brzozowski_mem', D_union] at *
+    rw [ih]
+}
+
+lemma brzozowski_not_mem'_union_iff(R₁ R₂ : Regex 𝒜) (w : Word 𝒜):
+  w ∉ (R₁ ⋃ R₂) ↔ w ∉ R₁ ∧ w ∉ R₂
+:= by simp [brzozowski_mem'_union_iff]; tauto
+
+lemma brzozowski_mem'_empty_not_in_D_delta(c: 𝒜)(R: Regex 𝒜):
+  [] ∉ 𝒟 c (δ R)
+:= by {
+  simp [Membership.mem, brzozowski_mem', νB_correct]
+  simp [D_delta_language]
+  tauto
+}
+
+lemma brzozowski_not_mem'_D_delta (c: 𝒜)(w: Word 𝒜) (R: Regex 𝒜):
+  w ∉ 𝒟 c (δ R)
+:= by {
+  induction' w with b x ih generalizing R
+  case nil =>
+    exact brzozowski_mem'_empty_not_in_D_delta c R
+  . sorry
+}
+
+lemma ss (R: Regex 𝒜) (w: Word 𝒜) (a: 𝒜):
+  a :: x ∉ δ R
+:= by {
+  induction R with
+  | empty | token _ =>
+    simp [δ]
+    apply brzozowski_mem'_empty
+  | concatenation e₁ e₂ ih₁ ih₂ =>
+    simp [δ_concatenation, brzozowski_mem'_cons, brzozowski_mem'_union_iff]
+    push_neg
+    constructor
+    . sorry
+    . sorry
+  | union e₁ e₂ ih₁ ih₂ =>
+    simp [δ_union]
+    rw [brzozowski_mem'_union_iff]
+    push_neg
+    exact ⟨ ih₁, ih₂⟩
+  | star e ih =>
+    simp [δ_star]
+    sorry
+}
+
+lemma brzozowski_mem'_delta(R: Regex 𝒜) (w: Word 𝒜):
+  w ∈ δ R ↔ w = [] ∧ [] ∈ R
+:= by {
+  induction' w with a x ih generalizing R
+  case nil =>
+    simp [Membership.mem, brzozowski_mem'] at *
+    induction R with
+    | empty | token _ => tauto
+    | concatenation e₁ e₂ ih₁ ih₂ =>
+      simp [D_concatenation, brzozowski_mem'_union_iff] at *
+      tauto
+    | union e₁ e₂ ih₁ ih₂ =>
+      simp [D_union, brzozowski_mem'_union_iff] at *
+      tauto
+    | star e ih =>
+      simp [D_star, brzozowski_mem'_union_iff] at *
+  . simp [brzozowski_mem'_cons]
+    sorry
+}
+
+lemma brzozowski_mem'_concat_iff(R₁ R₂ : Regex 𝒜) (w : Word 𝒜) :
+  w ∈ (R₁ ⋅ R₂) ↔ ∃ w₁ w₂, w₁ ++ w₂ = w ∧ w₁ ∈ R₁ ∧ w₂ ∈ R₂
+:= by {
+  induction' w with a x ih generalizing R₁ R₂
+  case nil =>
+    simp [Membership.mem, brzozowski_mem'_empty, brzozowski_mem', D_concatenation]
+    constructor
+    . intro H
+      exists []
+      exists []
+    . rintro ⟨ w₁, w₂, hw, hm₁, hm₂⟩
+      simp [nil_append_nil] at hw
+      rw [hw.1] at hm₁
+      rw [hw.2] at hm₂
+      simp [brzozowski_mem'] at *
+      exact And.intro hm₁ hm₂
+  . rw [brzozowski_mem'_cons, D_concatenation]
+    rw [brzozowski_mem'_union_iff]
+    constructor
+    . rw [ih, ih]
+      rintro (⟨w₁, w₂, hw, hm₁, hm₂⟩ | ⟨w₁, w₂, hw, hm₁, hm₂⟩)
+      . exists a::w₁
+        exists w₂
+        exact ⟨by rw [←hw, List.cons_append], hm₁, hm₂⟩
+      . exists []
+        exists (a::w₂)
+        have hδ: w₁ ∈ δ R₁ ↔ w₁ = [] ∧ [] ∈ R₁ := by {
+          exact brzozowski_mem'_delta R₁ w₁
+        }
+        rw [hδ] at hm₁
+        constructor
+        . rw [hm₁.1] at hw
+          rw [nil_append_word, List.cons_inj] at *
+          exact hw
+        . constructor
+          . exact hm₁.2
+          . exact hm₂
+    . intro H
+      rw [ih, ih]
+      rcases H with ⟨w₁, w₂, hw, hm₁, hm₂⟩
+      by_cases h: [] ∈ R₁
+      . --[] ∈ ℒ R₁
+        cases' w₁ with b t
+        . --w₂ = []
+          right
+          rw [List.nil_append] at hw
+          rw [hw] at hm₂
+          exists []
+          exists x
+          constructor
+          . tauto
+          . constructor
+            . -- this disappears since [] in ℒ R₁ -> [] ∈ νB δ R₁
+              have hδ: [] ∈ δ R₁ ↔ [] ∈ R₁ := by {
+                rw [brzozowski_mem'_delta]
+                tauto
+              }
+              exact hδ.2 hm₁
+            . exact hm₂
+        . --w₂ = b::t
+          left
+          rw [List.cons_append, List.cons_eq_cons] at hw
+          refine' ⟨t, w₂, hw.2, _, hm₂⟩
+          rw [←hw.1]
+          exact hm₁
+      . --[] ∉ ℒ R₁
+        left
+        cases' w₁ with b t
+        · --rw [Membership.mem, brzozowski_mem', νB_correct] at hm₁
+          contradiction
+        · rw [List.cons_append, List.cons_eq_cons] at hw
+          refine' ⟨t, w₂, hw.2, _, hm₂⟩
+          rw [←hw.1]
+          exact hm₁
+}
+
+lemma brzozowski_not_mem'_empty_concat (w : Word 𝒜) (R: Regex 𝒜):
+  w ∉ (Φ ⋅ R)
+:= by {
+  induction w generalizing R
+  case nil => simp [Membership.mem, brzozowski_mem']
+  case cons c w ih =>
+    rw [brzozowski_mem'_cons, D_concatenation]
+    rw [brzozowski_not_mem'_union_iff]
+    constructor
+    . rw [D_empty]
+      apply ih
+    . rw [δ_empty]
+      apply ih
+}
+
+lemma brzozowski_not_mem'_empty_concat_right (w : Word 𝒜) (R: Regex 𝒜):
+  w ∉ (R ⋅ Φ)
+:= by {
+  induction w generalizing R
+  case nil => simp [Membership.mem, brzozowski_mem']
+  case cons c w ih =>
+    simp [] at *
+    rw [brzozowski_mem'_cons, D_concatenation]
+    rw [D_empty]
+    rw [brzozowski_not_mem'_union_iff]
+    constructor
+    . apply ih
+    . apply ih
+}
+
+lemma brzozowski_mem'_char_iff(w: Word 𝒜):
+  w ∈ (τ c: Regex 𝒜) ↔ w = [c]
+:= by {
+  cases' w with h t
+  . simp [Membership.mem, brzozowski_mem']
+  cases' t with h₁ t
+  . simp [Membership.mem, brzozowski_mem']
+    split_ifs
+    . tauto
+    . rw [List.singleton_inj]; tauto
+  . constructor
+    . rw [List.cons.injEq]
+      intro H
+      exfalso
+      rw [brzozowski_mem'_cons, brzozowski_mem'_cons] at H
+      rw [D_token] at H
+      split_ifs at H
+      . rw [D_eps] at H
+        simp [brzozowski_not_mem'_empty_concat] at H
+      . rw [D_empty] at H
+        simp [brzozowski_mem'_empty] at H
+    . rw [List.cons.injEq]
+      simp [*]
+}
+
+lemma brzozowski_mem'_char_delta_regex_iff(c: 𝒜)(R: Regex 𝒜):
+  [c] ∉ (δ R)
+:= by {
+  simp [brzozowski_mem'_cons]
+  apply brzozowski_mem'_empty_not_in_D_delta
+}
+
+lemma brzozowski_mem'_eps(w: Word 𝒜):
+  w ∈ (ε: Regex 𝒜) ↔ w = []
+:= by {
+  induction w with
+  | nil => simp [Membership.mem, brzozowski_mem'] at *
+  | cons c w =>
+    simp [ brzozowski_mem', νB] at *
+    apply brzozowski_not_mem'_empty_concat
+}
+
+lemma brzozowski_mem'_d_delta (c: 𝒜)(w: Word 𝒜)(r₁ r₂: Regex 𝒜):
+  w ∉ (𝒟 c (δ r₁)) → w ∉ (𝒟 c (δ r₁)⋅r₂)
+:= by {
+  intro H
+  induction' w generalizing r₁ r₂
+  case nil =>
+    simp [Membership.mem, brzozowski_mem', brzozowski_mem'_empty, νB_correct] at *
+    rw [D_delta_language] at *
+    intro H₁
+    exfalso
+    contradiction
+  case cons c₁ w ih =>
+    rw [brzozowski_mem'_cons] at *
+    sorry
+}
+
+
+
+lemma brzozowski_mem'_delta_iff(w: Word 𝒜)(R: Regex 𝒜):
+  w ∈ (δ R) ↔ w = [] ∧ [] ∈ ℒ R
+:= by {
+  induction w generalizing R
+  case nil =>
+    simp [Membership.mem, brzozowski_mem', νB_correct]
+    exact ε_in_δ_ε_in_r
+  case cons h t ih =>
+    simp
+    rw [brzozowski_mem'_cons]
+    intro H
+    exfalso
+    -- simp [brzozowski_mem'] at *
+    induction R --generalizing t
+    case empty =>
+      simp [δ_empty,brzozowski_mem'_empty] at *
+    case token ch =>
+      simp [δ_token, brzozowski_mem'_empty] at *
+    case concatenation e₁ e₂ ih₁ ih₂ =>
+      sorry
+    case union e₁ e₂ ih₁ ih₂ =>
+      simp [δ_union, brzozowski_mem'_union_iff,  brzozowski_mem'_empty] at *
+      rcases  H with H₁ | H₂
+      . apply ih₁ H₁
+      . apply ih₂ H₂
+    case star e _ =>
+      simp [δ_star, brzozowski_mem'_empty] at *
+      simp [brzozowski_not_mem'_empty_concat] at *
+}
+
+
+
+lemma brzozowski_mem'_star_iff(w: Word 𝒜) (R: Regex 𝒜):
+  w ∈ (R★) ↔ ∃ a w₁, a::w₁ = w ∧ ([a] ∈ R) ∧ (w₁ ∈ (R★))
+:= by {
+  simp [brzozowski_mem'_cons]
+  induction R with
+  | empty =>
+    sorry
+
+  | token ch => sorry
+  | concatenation e₁ e₂ ih₁ ih₂ => sorry
+  | union e₁ e₂ ih₁ ih₂ => sorry
+  | star e ih => sorry
+}
+
+-- it should be computable when we remove all the sorrys
+noncomputable instance mem.decidable : ∀ (w : Word 𝒜) (R : Regex 𝒜), Decidable (w ∈ R)
+  | w, Φ => isFalse $ brzozowski_mem'_empty w
+  | w, τ t => by rw [brzozowski_mem'_char_iff]; tauto
+  | w, e₁ ⋅ e₂ => by rw [brzozowski_mem'_concat_iff]; tauto
+  | w, e₁ ⋃ e₂ => by rw [brzozowski_mem'_union_iff]; tauto
+  | w, e★ => by rw [brzozowski_mem'_star_iff]; tauto
+
+example: [2, 3] ∈ ((τ 2 ⋅ τ 3): Regex ℕ) := rfl
+
+lemma ε_in_e_then_δ_eq_ε(e: Regex 𝒜): [] ∈ ℒ e → ℒ (δ e) = 1 := by {
+  intro H
+  rw [δ_eq_ν]
+  rwa [ν_eq_one_iff]
+}
+
+-- @[simp]
+theorem mem_regex_iff_mem_language_regex (w : Word 𝒜)(R : Regex 𝒜):
+  w ∈ R ↔ w ∈ ℒ R
+:= by {
+  induction R --generalizing wx
+  case empty => simp [brzozowski_mem'_empty]; tauto
+  case token => simp [brzozowski_mem'_char_iff]
+  case concatenation r₁ r₂ ih₁ ih₂ =>
+    simp [brzozowski_mem'_concat_iff];
+    sorry
+  case union => {
+    simp [ℒ]
+    sorry
+  }
+  case star => {
+    simp [ℒ]
+    sorry
+  }
+}
+
+noncomputable instance (r: Regex 𝒜): DecidablePred (· ∈ ℒ r) := fun _ ↦
+  decidable_of_iff _ (mem_regex_iff_mem_language_regex _ _)
+
+-- #reduce ([2, 3] ∈ ((τ 2 ⋅ τ 3): Regex ℕ))
+-- #eval ([2, 3] ∈ ((τ 2 ⋅ τ 3): Regex ℕ))
